lz78/LZ_Tokens.v
@@ -1,88 +1,100 @@
 From Stdlib Require Import Arith Strings.Byte List Lia.
-Require Import Utils LZ_Dict.
+Require Import Utils.
+Require Import LZ_Dict.
 Import ListNotations.
+Require Import BinPos.
 
 Module Tokens.
 
   Inductive Token :=
-    | Tok (index: nat) (next: byte)
-    | Last (index: nat).
+    | Tok (index: nat) (phr : list bool) (next: bool)
+    | Last (index: nat) (phr : list bool).
 
   Fixpoint valid_tokens (tokens: list Token) (dict_size: nat) :=
     match tokens with
-    | Tok index _ :: rest => index < 256 ^ (num_bytes_for_dict dict_size)
+    | Tok index _ _ :: rest => index < 2 ^ (num_bits_for_dict dict_size)
                                /\ valid_tokens rest (S dict_size)
-    | Last _ :: _ :: _ => False
-    | [Last index] => index < 256 ^ (num_bytes_for_dict dict_size) 
+    | Last _ _ :: _ :: _  => False
+    | [Last index _] => index < 2 ^ (num_bits_for_dict dict_size) 
     | [] => True
     end.
 
-  Definition nat_to_byte (n: nat): byte :=
+  (* Search (Pos.to_nat _). *)
+
+  Fixpoint nat_to_k_bits (k n : nat) : list bool :=
+    match k with
+      | 0 => []
+      | S t => (if (n mod 2) =? 0 then false else true) :: nat_to_k_bits t (n / 2)
+    end.
+
+  Definition to_nat (b : bool) : nat :=
+    match b with
+      | true => 1
+      | false => 0
+    end.
+
+  Fixpoint k_bits_to_nat (bits: list bool) :=
+    match bits with
+    | [] => 0
+    | b :: rest => to_nat b + 2 * k_bits_to_nat rest
+    end.
+      
+  (* Definition nat_to_byte (n: nat): byte :=
     match of_nat (n mod 256) with
     | Some b => b
     | None => x00 (* Never happens *)
-    end.
+    end. *)
 
-  Fixpoint nat_to_k_bytes (k n: nat) :=
+  (* Fixpoint nat_to_k_bytes (k n: nat) :=
     match k with
     | 0 => []
     | S k => nat_to_byte (n mod 256) :: nat_to_k_bytes k (n / 256)
-    end.
+    end. *)
 
-  Fixpoint k_bytes_to_nat (bytes: list byte) :=
+  (* Fixpoint k_bytes_to_nat (bytes: list byte) :=
     match bytes with
     | [] => 0
     | b :: rest => to_nat b + 256 * k_bytes_to_nat rest
-    end.
+    end. *)
 
-  Fixpoint tokens_to_bytes' (dict_size: nat) (tokens: list Token) :=
+  Fixpoint tokens_to_bits' (dict_size: nat) (tokens: list Token) :=
     match tokens with
     | [] => []
-    | Tok index next :: rest =>
-        nat_to_k_bytes (num_bytes_for_dict dict_size) index ++ [next] ++
-        tokens_to_bytes' (S dict_size) rest
-    | Last index :: _ =>
-        nat_to_k_bytes (num_bytes_for_dict dict_size) index
+    | Tok index phr next :: rest =>
+        nat_to_k_bits (num_bits_for_dict dict_size) index ++ [next] ++
+        tokens_to_bits' (S dict_size) rest
+    | Last index _ :: _ =>
+        nat_to_k_bits (num_bits_for_dict dict_size) index
     end.
 
-  Definition tokens_to_bytes (tokens: list Token) :=
-    tokens_to_bytes' 1 tokens.
+  Definition tokens_to_bits (tokens: list Token) :=
+    tokens_to_bits' 1 tokens.
 
-  Fixpoint bytes_to_tokens' (fuel dict_size: nat) (bytes: list byte) :=
-    match fuel, bytes with
+  Fixpoint bits_to_tokens' (fuel dict_size: nat) (bits: list bool) : list Token :=
+    match fuel, bits with
     | 0, _ => []
     | _, [] => []
     | S fuel, _ =>
-        let k := num_bytes_for_dict dict_size in
-        if length bytes <? k then []
-        else if length bytes =? k then [Last (k_bytes_to_nat bytes)]
+        let k := num_bits_for_dict dict_size in
+        if length bits <? k then []
+        else if length bits =? k then [Last (k_bits_to_nat bits) []]
         else
-          let index_bytes := firstn k bytes in
-          match skipn k bytes with
-          | [] => [Last (k_bytes_to_nat index_bytes)]
+          let index_bits := firstn k bits in
+          match skipn k bits with
+          | [] => [Last (k_bits_to_nat index_bits) []]
           | next :: rest =>
-              Tok (k_bytes_to_nat index_bytes) next :: bytes_to_tokens' fuel (S dict_size) rest
+              Tok (k_bits_to_nat index_bits) [] next :: (bits_to_tokens' fuel (S dict_size) rest)
           end
     end.
 
-  Definition bytes_to_tokens (bytes: list byte) :=
-    bytes_to_tokens' (length bytes) 1 bytes.
+  Definition bits_to_tokens (bits: list bool) :=
+    bits_to_tokens' (length bits) 1 bits.
 
-
-  Lemma nat_to_byte_correctness: forall n,
-    n < 256 ->
-    to_nat (nat_to_byte n) = n.
+  Lemma nat_to_bit_correctness: forall n,
+    n < 2 ->
+    to_nat (if n =? 0 then false else true) = n.
   Proof.
-    unfold nat_to_byte.
-    intros.
-    destruct (of_nat (_ mod 256)) eqn:?.
-    - apply to_of_nat_iff.
-      rewrite (Nat.mod_small n 256 ltac:(lia)) in Heqo.
-      assumption.
-    - exfalso.
-      apply of_nat_None_iff in Heqo.
-      pose proof (Nat.mod_upper_bound n 256 ltac:(lia)).
-      lia.
+    intros. destruct n. simpl. reflexivity. destruct n. simpl. reflexivity. lia.
   Qed.
 
   Arguments Nat.modulo : simpl never.
@@ -91,16 +103,16 @@ Module Tokens.
   Arguments Nat.div : simpl never.
   Arguments Nat.mul : simpl never.
 
-  Lemma nat_to_k_bytes_correctness: forall k n,
-    n < 256 ^ k ->
-    k_bytes_to_nat (nat_to_k_bytes k n) = n.
+  Lemma nat_to_k_bits_correctness: forall k n,
+    n < 2 ^ k ->
+    k_bits_to_nat (nat_to_k_bits k n) = n.
   Proof.
     induction k; simpl; intros n Hnlt.
     - rewrite Nat.pow_0_r in Hnlt.
       lia.
     - rewrite IHk.
-      + rewrite nat_to_byte_correctness.
-        * pose proof (Nat.div_mod_eq n 256).
+      + rewrite nat_to_bit_correctness with (n := n mod 2).
+        * pose proof (Nat.div_mod_eq n 2).
           lia.
         * apply Nat.mod_upper_bound.
           lia.
@@ -109,19 +121,36 @@ Module Tokens.
         lia.
   Qed.
 
-  Lemma nat_to_k_bytes_length: forall k n,
-    length (nat_to_k_bytes k n) = k.
+  Lemma nat_to_k_bits_length: forall k n,
+    length (nat_to_k_bits k n) = k.
   Proof.
     induction k; simpl; intros.
     - reflexivity.
     - now rewrite IHk.
   Qed.
 
-  Lemma tokens_to_bytes_correctness': forall fuel tokens dict_size bytes,
-    length bytes <= fuel ->
+  Definition token_equiv (t1 t2 : Token) :=
+    match (t1, t2) with
+      | (Tok _ _ _, Last _ _) => False
+      | (Last _ _, Tok _ _ _) => False
+      | (Tok ind1 _ next1, Tok ind2 _ next2) => ind1 = ind2 /\ next1 = next2
+      | (Last ind1 _, Last ind2 _) => ind1 = ind2
+    end.
+
+  Fixpoint list_eq {A : Type} (eqb : A -> A -> Prop) (s t : list A) : Prop :=
+    match (s, t) with
+    | (cons s1 s2, cons t1 t2) => (eqb s1 t1) /\ (list_eq eqb s2 t2)
+    | (nil, nil) => True
+    | _ => False
+    end.
+  
+  Print token_equiv.
+
+  Lemma tokens_to_bits_correctness': forall fuel tokens dict_size bits,
+    length bits <= fuel ->
     valid_tokens tokens dict_size ->
-    tokens_to_bytes' dict_size tokens = bytes ->
-    bytes_to_tokens' fuel dict_size bytes = tokens.
+    tokens_to_bits' dict_size tokens = bits ->
+    list_eq token_equiv (bits_to_tokens' fuel dict_size bits) (tokens).
   Proof.
     induction fuel; simpl; intros.
     - destruct tokens. reflexivity.
@@ -132,50 +161,50 @@ Module Tokens.
       + apply app_eq_nil in H3.
         destruct H3.
         discriminate.
-      + pose proof (num_bytes_for_dict_gt_one dict_size).
-        destruct (num_bytes_for_dict dict_size).
+      + pose proof (num_bits_for_dict_gt_one dict_size).
+        destruct (num_bits_for_dict dict_size).
         * lia.
         * simpl in H3.
           discriminate.
-    - destruct bytes.
+    - destruct bits.
       + destruct tokens. reflexivity.
         destruct t; simpl in H1.
         * apply app_eq_nil in H1.
           destruct H1.
           discriminate.
-        * pose proof (num_bytes_for_dict_gt_one dict_size).
-          destruct (num_bytes_for_dict dict_size).
+        * pose proof (num_bits_for_dict_gt_one dict_size).
+          destruct (num_bits_for_dict dict_size).
           -- lia.
           -- simpl in H1.
              discriminate.
-      + destruct (length (b :: bytes) <? num_bytes_for_dict dict_size) eqn:?.
+      + destruct (length (b :: bits) <? num_bits_for_dict dict_size) eqn:?.
         * destruct tokens. reflexivity.
           simpl in H1.
           apply Nat.ltb_lt in Heqb0.
           destruct t.
-          -- pose proof (nat_to_k_bytes_length (num_bytes_for_dict dict_size) index).
-             assert (length (nat_to_k_bytes (num_bytes_for_dict dict_size) index)
-                      <= length (b :: bytes)). {
+          -- pose proof (nat_to_k_bits_length (num_bits_for_dict dict_size) index).
+             assert (length (nat_to_k_bits (num_bits_for_dict dict_size) index)
+                      <= length (b :: bits)). {
                rewrite <- H1, length_app.
                lia.
              }
              lia.
-          -- pose proof (nat_to_k_bytes_length (num_bytes_for_dict dict_size) index).
+          -- pose proof (nat_to_k_bits_length (num_bits_for_dict dict_size) index).
              rewrite H1 in H2.
              lia.
-        * destruct (length (b :: bytes) =? num_bytes_for_dict dict_size) eqn:?.
+        * destruct (length (b :: bits) =? num_bits_for_dict dict_size) eqn:?.
           -- destruct tokens; simpl in H1.
              ++ discriminate.
              ++ destruct t.
                 ** apply Nat.eqb_eq in Heqb1.
-                   rewrite <- H1, length_app, nat_to_k_bytes_length in Heqb1.
+                   rewrite <- H1, length_app, nat_to_k_bits_length in Heqb1.
                    simpl in Heqb1. lia.
                 ** destruct tokens.
-                   --- rewrite <- H1, nat_to_k_bytes_correctness.
-                       +++ reflexivity.
+                   --- rewrite <- H1, nat_to_k_bits_correctness.
+                       +++ simpl. unfold token_equiv. auto.
                        +++ now simpl in H0.
                    --- simpl in H0. now exfalso.
-          -- destruct (skipn (num_bytes_for_dict dict_size) (b :: bytes)) eqn:?.
+          -- destruct (skipn (num_bits_for_dict dict_size) (b :: bits)) eqn:?.
              ++ apply Nat.ltb_ge in Heqb0.
                 apply Nat.eqb_neq in Heqb1.
                 apply skipn_all_iff in Heql.
@@ -184,12 +213,12 @@ Module Tokens.
                 ** discriminate.
                 ** destruct t.
                    --- f_equal.
-                       +++ pose proof (firstn_skipn (num_bytes_for_dict dict_size) (b :: bytes)).
+                       +++ pose proof (firstn_skipn (num_bits_for_dict dict_size) (b :: bits)).
                            rewrite Heql in H2.
                            rewrite <- H2 in H1.
-                           assert (firstn (num_bytes_for_dict dict_size) (b :: bytes)
-                                   = nat_to_k_bytes (num_bytes_for_dict dict_size) index). {
-                             pose proof (nat_to_k_bytes_length (num_bytes_for_dict dict_size) index).
+                           assert (firstn (num_bits_for_dict dict_size) (b :: bits)
+                                   = nat_to_k_bits (num_bits_for_dict dict_size) index). {
+                             pose proof (nat_to_k_bits_length (num_bits_for_dict dict_size) index).
                              eapply app_l_eq_length in H1.
                              - congruence.
                              - rewrite H3.
@@ -197,18 +226,23 @@ Module Tokens.
                              - rewrite length_firstn.
                                apply Nat.ltb_ge in Heqb0.
                                apply Nat.eqb_neq in Heqb1.
-                               assert (Nat.min (num_bytes_for_dict dict_size) (length (b :: bytes))
-                                       = num_bytes_for_dict dict_size) by lia.
+                               assert (Nat.min (num_bits_for_dict dict_size) (length (b :: bits))
+                                       = num_bits_for_dict dict_size) by lia.
                                now rewrite H4.
                            }
                            rewrite H3 in H1 |- *.
-                           rewrite nat_to_k_bytes_correctness.
+                           rewrite nat_to_k_bits_correctness.
                            *** f_equal.
                                apply app_inv_head in H1.
-                               congruence.
+                               
+                               simpl. split. 
+                                ---- unfold token_equiv. split.
+                                  **** reflexivity.
+                                  **** congruence.
+                                ---- simpl. admit. 
                            *** simpl in H0.
                                now destruct H0.
-                       +++ erewrite IHfuel.
+                       (* +++ erewrite IHfuel.
                            *** reflexivity.
                            *** pose proof (length_skipn (num_bytes_for_dict dict_size) (b :: bytes)).
                                rewrite Heql in H2.
@@ -221,19 +255,19 @@ Module Tokens.
                                rewrite <- H2 in Heql at 1.
                                rewrite skipn_app, Nat.sub_diag, skipn_all, skipn_0 in Heql.
                                simpl in Heql.
-                               congruence.
-                   --- pose proof (nat_to_k_bytes_length (num_bytes_for_dict dict_size) index).
+                               congruence. *)
+                   --- pose proof (nat_to_k_bits_length (num_bits_for_dict dict_size) index).
                        rewrite H1 in H2.
                        apply Nat.eqb_neq in Heqb1.
                        lia.
-  Qed.
+  Admitted.
 
-  Lemma tokens_to_bytes_correctness: forall tokens,
+  Lemma tokens_to_bits_correctness: forall tokens,
     valid_tokens tokens 1 ->
-    bytes_to_tokens (tokens_to_bytes tokens) = tokens.
+    list_eq token_equiv (bits_to_tokens (tokens_to_bits tokens)) tokens.
   Proof.
     intros.
-    eapply tokens_to_bytes_correctness'.
+    eapply tokens_to_bits_correctness'.
     - lia.
     - assumption.
     - reflexivity.
@@ -241,7 +275,7 @@ Module Tokens.
   
   Lemma length_nat_to_k_bytes :
     forall k n,
-      length (nat_to_k_bytes k n) = k.
+      length (nat_to_k_bits k n) = k.
   Proof.
     induction k; simpl; intros; auto.
   Qed.
